defined a toy assembly langage

ASM/ASM.v
@@ -12,7 +12,7 @@ Require Export DoOption.
 
 Module Instruction : INSTRUCTION.
 
-  Inductive register: Type :=
+  Inductive register': Type :=
   | REG1
   | REG2
   | REG3
@@ -22,6 +22,7 @@ Module Instruction : INSTRUCTION.
   | REG7
   | REG8.
 
+  Definition register := register'.
 
   Definition register_eq_dec  (r1 r2: register): {r1 = r2}+{r1 <> r2}.
   Proof.
@@ -29,14 +30,17 @@ Module Instruction : INSTRUCTION.
   Qed.
 
 
-  Inductive instruction : Type :=
-  | Instr_noop: instruction
-  | Instr_and: register -> word -> register -> instruction
-  | Instr_direct_jump: word -> instruction
-  | Instr_direct_cond_jump: register -> word -> instruction
-  | Instr_indirect_jump: register -> instruction
-  | Instr_os_call: word -> instruction.
+  Inductive instruction' : Type :=
+  | Instr_noop: instruction'
+  | Instr_and: register -> word -> register -> instruction'
+  | Instr_read: register -> register -> instruction'
+  | Instr_write: register -> register -> instruction'
+  | Instr_direct_jump: word -> instruction'
+  | Instr_direct_cond_jump: register -> word -> instruction'
+  | Instr_indirect_jump: register -> instruction'
+  | Instr_os_call: word -> instruction'.
 
+  Definition instruction := instruction'.
 
   Open Scope nat_scope.
 
@@ -69,17 +73,25 @@ Module Instruction : INSTRUCTION.
         do reg2 <- reg_from_byte reg_code2;
           (* we assume a little endian processor *)
         Some (Instr_and reg1 (W b4 b3 b2 b1) reg2, 7)
-      | (HB0, HB2) ::: b1 ::: b2 ::: b3 ::: b4 ::: _ =>
+      | (HB0, HB2) ::: reg_code1 ::: reg_code2 ::: _ =>
+        do reg1 <- reg_from_byte reg_code1;
+        do reg2 <- reg_from_byte reg_code2;
+        Some (Instr_read reg1 reg2, 3)
+      | (HB0, HB3) ::: reg_code1 ::: reg_code2 ::: _ =>
+        do reg1 <- reg_from_byte reg_code1;
+        do reg2 <- reg_from_byte reg_code2;
+        Some (Instr_write reg1 reg2, 3)
+      | (HB0, HB4) ::: b1 ::: b2 ::: b3 ::: b4 ::: _ =>
         Some (Instr_direct_jump (W b4 b3 b2 b1), 5)
-      | (HB0, HB3) ::: reg_code1 ::: b1 ::: b2 ::: b3 ::: b4 ::: _ =>
+      | (HB0, HB5) ::: reg_code1 ::: b1 ::: b2 ::: b3 ::: b4 ::: _ =>
         do reg1 <- reg_from_byte reg_code1;
           (* we assume a little endian processor *)
         Some (Instr_direct_cond_jump reg1 (W b4 b3 b2 b1), 6)
-      | (HB0, HB4) ::: reg_code1 :::  _ =>
+      | (HB0, HB6) ::: reg_code1 :::  _ =>
         do reg1 <- reg_from_byte reg_code1;
           (* we assume a little endian processor *)
         Some (Instr_indirect_jump reg1, 2)
-      | (HB0, HB5) ::: _ =>
+      | (HB0, HB7) ::: _ =>
         Some (Instr_os_call (W byte0 byte0 byte0 byte0), 1)
       | _ => None
     end.
@@ -99,7 +111,13 @@ Module Instruction : INSTRUCTION.
       |  fst_Case_tac "fun_ind_parse_instr 9"
       |  fst_Case_tac "fun_ind_parse_instr 10"
       |  fst_Case_tac "fun_ind_parse_instr 11"
-      |  fst_Case_tac "fun_ind_parse_instr 12"].
+      |  fst_Case_tac "fun_ind_parse_instr 12"
+      |  fst_Case_tac "fun_ind_parse_instr 13"
+      |  fst_Case_tac "fun_ind_parse_instr 14"
+      |  fst_Case_tac "fun_ind_parse_instr 15"
+      |  fst_Case_tac "fun_ind_parse_instr 16"
+      |  fst_Case_tac "fun_ind_parse_instr 17"
+      |  fst_Case_tac "fun_ind_parse_instr 18"].
 
 
   Ltac fun_ind_parse_instr :=
@@ -119,6 +137,11 @@ Module Instruction : INSTRUCTION.
     fun_ind_parse_instr; simpl; clean; try omega.
   Qed.
 
+  Lemma inv_ll_cons: forall X (x1:X) l1 x2 l2,
+    tag_to_inv (ll_cons x1 l1 = ll_cons x2 l2).
+  Proof. constructor. auto. Qed.
+  Hint Rewrite inv_ll_cons: opt_inv.
+
 
   Lemma parse_instruction_only_read:
     forall ll instr n, parse_instruction ll = Some (instr, n) ->
@@ -127,22 +150,148 @@ Module Instruction : INSTRUCTION.
       parse_instruction ll' = Some (instr, n).
   Proof.
     intros.
-    fun_ind_parse_instr; simpl in *; clean.
-    Case "fun_ind_parse_instr 2".
+    fun_ind_parse_instr; simpl in *; clean; simpl in *;    
+    repeat match goal with
+      | H : context [match ?l with
+                       | ll_nil => _
+                       | ll_cons _ _ => _
+                     end] |- _ =>
+      destruct l as [|? []]; clean
+    end; simpl in *; try (rewrite e0); try (rewrite e1); auto.
+  Qed.
     
 
   Lemma size_instr_not_0: forall ll instr n,
     parse_instruction ll = Some (instr, n) -> n <> O.
+  Proof.
+    intros.
+    fun_ind_parse_instr; simpl in *; clean; simpl in *; auto.
+  Qed.
 
   Lemma size_instr_inf_max_size: forall ll instr n,
-    parse_instruction ll = Some (instr, n) -> (n < instr_max_size)%nat.
+    parse_instruction ll = Some (instr, n) -> (n <= instr_max_size)%nat.
+  Proof.
+    unfold instr_max_size. intros.
+    fun_ind_parse_instr; simpl in *; clean; simpl in *; auto;omega.
+  Qed.
 
 
-  Lemma classify_instruction: instruction -> instruction_classification register.
+  Definition classify_instruction instr :=
+    match instr with
+      | Instr_noop => OK_instr
+      | Instr_and reg1 w reg2 =>
+        if register_eq_dec reg1 reg2 then
+          Mask_instr reg1 w
+        else
+          OK_instr
+      | Instr_read _ _ => OK_instr
+      | Instr_write _ _ => OK_instr
+      | Instr_direct_jump w => Direct_jump w
+      | Instr_direct_cond_jump reg w => Direct_jump w
+      | Instr_indirect_jump reg => Indirect_jump reg
+      | Instr_os_call w => Invalid_instruction
+    end.
 
 
-  Lemma instruction_semantics: forall code_size:N, instruction ->
-    state register -> instruction_target_state register -> Prop.
+  Definition read_word (mem:memory) addr : option word :=
+    do b1 <- mem addr;
+    do b2 <- mem (addr + 1)%N;
+    do b3 <- mem (addr + 2)%N;
+    do b4 <- mem (addr + 3)%N;
+    Some (W b4 b3 b2 b1).
+
+  Definition write_byte (mem:memory) addr byte : memory:=
+    fun n =>
+      if N_eq_dec n addr then Some byte else mem n.
+
+  Definition write_word (mem:memory) addr w :=
+    match w with
+      | W b4 b3 b2 b1 =>
+        write_byte (write_byte (write_byte (write_byte mem addr b1) (addr + 1) b2)
+          (addr + 2) b3) (addr + 3) b4
+    end%N.
+
+  Lemma read_write_word: forall mem addr w,
+    read_word (write_word mem addr w) addr = Some w.
+  Proof.
+    intros.
+    unfold read_word, write_word, write_byte.
+    destruct w as [b4 b3 b2 b1].
+    repeat
+      match goal with
+        | |- context[N_eq_dec ?v1 ?v2] =>
+          destruct (N_eq_dec v1 v2); try (elimtype False; omega')
+      end.
+    reflexivity.
+  Qed.
+
+  Definition update_reg (regs: register -> word) reg w :=
+    fun r => if register_eq_dec r reg then w else regs r.
+
+Open Scope N_scope.
+
+  Inductive instruction_semantics' (code_size:N): instruction ->
+    state register -> instruction_target_state register -> Prop :=
+  | IS_noop: forall mem regs pc,
+    instruction_semantics' code_size Instr_noop
+    {| state_mem := mem;  state_regs := regs;  state_pc := pc |}
+    (Good_state {| state_mem := mem;
+                   state_regs := regs;
+                   state_pc := pc + 1|})
+  | IS_and: forall mem regs pc reg1 reg2 w,
+    instruction_semantics' code_size (Instr_and reg1 w reg2)
+    {| state_mem := mem;  state_regs := regs;  state_pc := pc |}
+    (Good_state {| state_mem := mem;
+                   state_regs := update_reg regs reg2 (word_and w (regs reg1));
+                   state_pc := pc + 7|})
+  | IS_read: forall mem regs pc reg1 reg2 addr w,
+    addr = N_of_word (regs reg1) ->
+    Some w = read_word mem addr ->
+    instruction_semantics' code_size (Instr_read reg1 reg2)
+    {| state_mem := mem;  state_regs := regs;  state_pc := pc |}
+    (Good_state {| state_mem := mem;
+                   state_regs := update_reg regs reg2 w;
+                   state_pc := pc + 3|})
+  | IS_write: forall mem regs pc reg1 reg2 addr,
+    addr = N_of_word (regs reg2) ->
+    (* we cannot write in the header !!! *)
+    (header_size + code_size <= addr)%N ->
+    instruction_semantics' code_size (Instr_write reg1 reg2)
+    {| state_mem := mem;  state_regs := regs;  state_pc := pc |}
+    (Good_state {| state_mem := write_word mem addr (regs reg1);
+                   state_regs := regs;
+                   state_pc := pc + 3|})
+  | IS_direct_jump: forall mem regs pc w,
+    instruction_semantics' code_size (Instr_direct_jump w)
+    {| state_mem := mem;  state_regs := regs;  state_pc := pc |}
+    (Good_state {| state_mem := mem;
+                   state_regs := regs;
+                   state_pc := N_of_word w |})
+  | IS_direct_cond_jump_yes: forall mem regs pc reg w,
+    regs reg <> word_of_N 0 ->
+    instruction_semantics' code_size (Instr_direct_cond_jump reg w)
+    {| state_mem := mem;  state_regs := regs;  state_pc := pc |}
+    (Good_state {| state_mem := mem;
+                   state_regs := regs;
+                   state_pc := N_of_word w |})
+  | IS_direct_cond_jump_no: forall mem regs pc reg w,
+    regs reg = word_of_N 0 ->
+    instruction_semantics' code_size (Instr_direct_cond_jump reg w)
+    {| state_mem := mem;  state_regs := regs;  state_pc := pc |}
+    (Good_state {| state_mem := mem;
+                   state_regs := regs;
+                   state_pc := pc + 6 |})
+  | IS_indirect_jump: forall mem regs pc reg,
+    instruction_semantics' code_size (Instr_indirect_jump reg)
+    {| state_mem := mem;  state_regs := regs;  state_pc := pc |}
+    (Good_state {| state_mem := mem;
+                   state_regs := regs;
+                   state_pc := N_of_word (regs reg)|})
+  | IS_os_call: forall st w,
+    instruction_semantics' code_size (Instr_os_call w)
+    st Bad_state.
+
+  Definition instruction_semantics := instruction_semantics'.
 
 
   (* the first parameter is to indicate that the n first bytes of the memory
@@ -153,6 +302,20 @@ Module Instruction : INSTRUCTION.
   Lemma sem_no_overwrite: forall code_size instr st1 st2,
     instruction_semantics code_size instr st1 (Good_state st2) ->
     forall n', n' < header_size + code_size -> st1.(state_mem) n' = st2.(state_mem) n'.
+  Proof.
+    intros.
+    inv H; simpl; auto.
+    remember (N_of_word (regs reg2)) as n. clear Heqn.
+    unfold write_word, write_byte.
+    destruct (regs reg1) as [b4 b3 b2 b1].
+    repeat
+      match goal with
+        | |- context[N_eq_dec ?v1 ?v2] =>
+          destruct (N_eq_dec v1 v2); try (elimtype False; omega')
+      end.
+    reflexivity.
+  Qed.
+    
 
   (* the "good" instructions can get stuck but neverr lead to a "bad state" *)
 
@@ -160,7 +323,10 @@ Module Instruction : INSTRUCTION.
     classify_instruction instr <> Invalid_instruction ->
     forall code_size st,
       ~ instruction_semantics code_size instr st Bad_state.
-
+  Proof.
+    intros. intro.
+    inv H0. simpl in H. congruence.
+  Qed.
 
   Lemma sem_OK_instr_pc: forall bm instr size,
     parse_instruction bm = Some (instr, size) ->
@@ -168,6 +334,10 @@ Module Instruction : INSTRUCTION.
     forall code_size st1 st2,
     instruction_semantics code_size instr st1 (Good_state st2) ->
     st2.(state_pc) = st1.(state_pc) + (N_of_nat size).
+  Proof.
+    intros.
+    fun_ind_parse_instr; clean; inv H1; try reflexivity; inv H0.
+  Qed.
 
   Lemma sem_Mask_instr_pc: forall bm instr size,
     parse_instruction bm = Some (instr, size) ->
@@ -176,6 +346,13 @@ Module Instruction : INSTRUCTION.
     forall code_size st1 st2,
     instruction_semantics code_size instr st1 (Good_state st2) ->
     st2.(state_pc) = st1.(state_pc) + (N_of_nat size).
+  Proof.
+    intros.
+    fun_ind_parse_instr; clean; try inv H0.
+    inv H1; reflexivity.
+  Qed.
+
+
 
   Lemma sem_Mask_instr_reg: forall bm instr size,
     parse_instruction bm = Some (instr, size) ->
@@ -184,7 +361,16 @@ Module Instruction : INSTRUCTION.
     forall code_size st1 st2,
     instruction_semantics code_size instr st1 (Good_state st2) ->
     st2.(state_regs) reg = word_and w (st1.(state_regs) reg).
-
+  Proof.
+    intros.
+    fun_ind_parse_instr; clean; try solve [inv H0].
+    simpl in H0.
+    destruct (register_eq_dec a a0); subst.
+    inv H0.
+    inv H1. simpl. unfold update_reg.
+    destruct register_eq_dec; congruence.
+    inv H0.
+  Qed.
 
   Lemma sem_Direct_jump_pc: forall bm instr size,
     parse_instruction bm = Some (instr, size) ->
@@ -194,6 +380,17 @@ Module Instruction : INSTRUCTION.
     instruction_semantics code_size instr st1 (Good_state st2) ->
     st2.(state_pc) = st1.(state_pc) + (N_of_nat size) \/
     st2.(state_pc) = N_of_word w.
+  Proof.
+    intros.
+    fun_ind_parse_instr; clean; try solve [inv H0].
+    Case "fun_ind_parse_instr 3".
+    simpl in H0. destruct register_eq_dec in H0; inv H0.
+    Case "fun_ind_parse_instr 12".
+    inv H0. inv H1. auto.
+    Case "fun_ind_parse_instr 13".
+    inv H0. inv H1; auto.
+  Qed.
+    
 
   Lemma sem_Indirect_jump_pc: forall bm instr size,
     parse_instruction bm = Some (instr, size) ->
@@ -203,5 +400,15 @@ Module Instruction : INSTRUCTION.
     instruction_semantics code_size instr st1 (Good_state st2) ->
     st2.(state_pc) = st1.(state_pc) + (N_of_nat size) \/
     st2.(state_pc) = N_of_word (st1.(state_regs) reg).
+  Proof.
+    intros.
+    fun_ind_parse_instr; clean; try solve [inv H0].
+    Case "fun_ind_parse_instr 3".
+    simpl in H0. destruct register_eq_dec in H0; inv H0.
+    Case "fun_ind_parse_instr 15".
+    inv H0. inv H1; auto.
+  Qed.
+
+End Instruction.
 
 
